moving lemmas around

eNFA_Regex_Equivalence/Basic.lean
@@ -14,14 +14,48 @@ variable {α : Type u} [Fintype α] [DecidableEq α]
 
 set_option linter.unusedSectionVars false
 
+------------------------------------
+---------- Helpfull tools ----------
+------------------------------------
+
+def is_alone_in_set (set: Set ℕ) (n: ℕ):= set = { n }
+
 
 namespace εNFA
+
+-----------------------------------------
+---------- Automata Path Tools ----------
+-----------------------------------------
+
+variable {α : Type u} {σ : Type v} (M : εNFA α σ) {S : Set σ} {s t u : σ} {a : α}
+
+@[simp]
+def Path.steps [DecidableEq σ] {s t : σ} {x : List (Option α)} : M.Path s t x → List (σ × Option α × Prop)
+  | nil s => [(s, none, True)]
+  | cons _ _ _ c _ _ p => [(s, c, (t ∈ M.step s c))] ++ p.steps
+
+def Path.steps.states [DecidableEq σ] : List (σ × Option α × Prop) → List σ
+  | List.nil => []
+  | List.cons head tail => [head.1] ++ states tail
+
+def Path.steps.word [DecidableEq σ] : List (σ × Option α × Prop) → List (Option α)
+  | List.nil => []
+  | List.cons head tail => [head.2.1] ++ word tail
+
+@[simp]
+def Path.states [DecidableEq σ] {s t : σ} {x : List (Option α)} : M.Path s t x → List σ
+  | nil s => [s]
+  | cons _ _ _ _ _ _ p => [s] ++ p.states
+
+lemma sub_stepList_is_path (A : εNFA α ℕ) (qs qf : ℕ) (x : List (Option α)) (path: A.Path qs qf x)
+    (SL : List (ℕ × Option α × Prop)) (hSL: SL ≠ []) :
+    SL.IsInfix path.steps → ∃ subpath, subpath = A.Path (SL.head hSL).1 (SL.getLast hSL).1 := by
+    simp only [↓existsAndEq, implies_true]
 
 
 ---------------------------------------
 ---------- Automata Doubling ----------
 ---------------------------------------
-
 
 
 def to_0mod2 (A : εNFA α ℕ) : εNFA α ℕ := {
@@ -253,10 +287,9 @@ lemma accepts_iff_1mod2_accepts (A : εNFA α ℕ) (A' : εNFA α ℕ) (hA': A' 
     A.accepts = A'.accepts := accepts_iff_mod2_accepts A A' (Or.inr hA')
 
 
-------------------------------------------
----------- Automata Containment ----------
-------------------------------------------
-
+---------------------------------------
+---------- General Automata  ----------
+---------------------------------------
 
 def contains (A : εNFA α ℕ) (A' : εNFA α ℕ) :=
     ∀ (q : ℕ), ∀ (σ: Option α), A'.step q σ ⊆ A.step q σ
@@ -277,34 +310,707 @@ lemma path_if_contains (A : εNFA α ℕ) (A' : εNFA α ℕ) (h_contains: A.con
         exact A.isPath_append.mpr ⟨ t, h_step, h_induction ⟩
 
 
-
------------------------------------------
----------- Automata Path Tools ----------
------------------------------------------
-
-variable {α : Type u} {σ : Type v} (M : εNFA α σ) {S : Set σ} {s t u : σ} {a : α}
-
-@[simp]
-def Path.steps [DecidableEq σ] {s t : σ} {x : List (Option α)} : M.Path s t x → List (σ × Option α × Prop)
-  | nil s => [(s, none, True)]
-  | cons _ _ _ c _ _ p => [(s, c, (t ∈ M.step s c))] ++ p.steps
-
-def Path.steps.states [DecidableEq σ] : List (σ × Option α × Prop) → List σ
-  | List.nil => []
-  | List.cons head tail => [head.1] ++ states tail
-
-def Path.steps.word [DecidableEq σ] : List (σ × Option α × Prop) → List (Option α)
-  | List.nil => []
-  | List.cons head tail => [head.2.1] ++ word tail
-
-@[simp]
-def Path.states [DecidableEq σ] {s t : σ} {x : List (Option α)} : M.Path s t x → List σ
-  | nil s => [s]
-  | cons _ _ _ _ _ _ p => [s] ++ p.states
-
-lemma sub_stepList_is_path (A : εNFA α ℕ) (qs qf : ℕ) (x : List (Option α)) (path: A.Path qs qf x)
-    (SL : List (ℕ × Option α × Prop)) (hSL: SL ≠ []) :
-    SL.IsInfix path.steps → ∃ subpath, subpath = A.Path (SL.head hSL).1 (SL.getLast hSL).1 := by
-    simp only [↓existsAndEq, implies_true]
-
+lemma dont_go_nowhere (A : εNFA α ℕ) (hAempty : A.start = ∅) : A.accepts = 0 := by
+    simp [Language.zero_def]
+    rw [Set.eq_empty_iff_forall_notMem] at hAempty ⊢
+    intro x
+    by_contra!
+    obtain ⟨ s₁, _, _, h_s₁, _⟩ := A.mem_accepts_iff_exists_path.mp this
+    simp [hAempty] at h_s₁ -- contradiction
 end εNFA
+
+variable {α : Type u} [Fintype α] [DecidableEq α]
+
+
+def SingularStart  := 2
+def SingularAccept := 0
+
+def to_singular (A : εNFA α ℕ) : εNFA α ℕ := {
+    start  := { SingularStart }
+    accept := { SingularAccept }
+    step   := fun q c =>
+        let A' := A.to_1mod2
+        if q % 2 = 1 then
+            if q ∈ A'.accept && c = none then
+                A'.step q c ∪ { SingularAccept }
+            else
+                A'.step q c
+        else
+            if q = SingularStart && c = none then
+                A'.start
+            else
+                ∅
+    : εNFA α ℕ
+}
+
+
+def is_singular (A : εNFA α ℕ) :=
+    (∃s: ℕ, is_alone_in_set A.start s) ∧ (∃a: ℕ, is_alone_in_set A.accept a)
+
+lemma to_singular_contains (A: εNFA α ℕ): (to_singular A).contains A.to_1mod2 := by
+    unfold εNFA.contains
+    intro q σ
+    simp [to_singular, εNFA.to_1mod2]
+    split_ifs
+    all_goals simp only [subset_insert, subset_refl, empty_subset]
+
+
+lemma accepts_iff_singular_accepts (A : εNFA α ℕ) (A' : εNFA α ℕ) (hA': A' = to_singular A) :
+    A.accepts = A'.accepts := by
+    rw [@Language.ext_iff]
+    intro x
+    constructor
+    case mp =>
+        intro h_A_accepts_x
+        rw[@εNFA.mem_accepts_iff_exists_path] at h_A_accepts_x ⊢
+
+        obtain ⟨ s, a, x', hs, ha, hx', hApath⟩ := h_A_accepts_x
+        use SingularStart, SingularAccept, ([none] ++ x' ++ [none])
+
+        refine ⟨ by subst hA'; rfl, by subst hA'; rfl,
+            by simp only [List.nil_append, List.reduceOption_cons_of_none, List.reduceOption_append, List.reduceOption_nil, List.append_nil, hx']
+            , ?_ ⟩
+
+        have hfirst: Nonempty (A'.Path SingularStart (2*s + 1) [none]) := by
+            subst hA'
+            simp [to_singular, εNFA.to_1mod2, hs, SingularStart]
+
+        have hlast: Nonempty (A'.Path (2*a + 1) SingularAccept [none]) := by
+            subst hA'
+            simp [to_singular, εNFA.to_1mod2, ha, SingularAccept]
+
+        have hmiddle: Nonempty (A'.Path (2*s + 1) (2*a + 1) x') := by
+            subst hA'
+            have h_A_0mod2_path := (A.path_iff_1mod2_path A.to_1mod2 s a (2*s + 1) (2*a + 1) x' rfl rfl rfl).mp hApath
+            have hcontains := to_singular_contains A
+            apply εNFA.path_if_contains at hcontains
+            exact hcontains (2*s + 1) (2*a + 1) x' h_A_0mod2_path
+
+        apply A'.isPath_append.mpr; use (2*a + 1)
+        refine ⟨ ?_, hlast ⟩
+
+        apply A'.isPath_append.mpr; use (2*s + 1)
+
+    case mpr =>
+        intro h_A'_accepts_x
+        rw [A.accepts_iff_1mod2_accepts A.to_1mod2 rfl]
+
+        rw[@εNFA.mem_accepts_iff_exists_path] at h_A'_accepts_x ⊢
+        obtain ⟨ s', a', x', h_s'_start, h_a'_accept, h_x', hA'path ⟩ := h_A'_accepts_x
+
+        have h_s'_2: s' = SingularStart := by
+            subst hA'
+            simp [to_singular] at h_s'_start
+            exact h_s'_start
+
+        have h_a'_4: a' = SingularAccept := by
+            subst hA'
+            simp [to_singular] at h_a'_accept
+            exact h_a'_accept
+
+        subst h_s'_2
+        subst h_a'_4
+        clear h_s'_start h_a'_accept
+
+        obtain ⟨ hA'path ⟩ := hA'path
+        cases hA'path
+        case cons s σ y' h_step h_path_s_accept =>
+            simp [hA', to_singular, SingularStart, SingularAccept] at h_step
+            obtain ⟨ ⟨ _, h_σ_none ⟩ , h_s_start ⟩ := h_step
+
+            have first_transition_is_to_odd_state: s % 2 = 1:=
+                A.to_1mod2.if_1mod2_qs_is_1mod2 ⟨A, rfl⟩ s h_s_start
+
+            have h_temp: ∀ (q q': ℕ) (σ : Option α), (q % 2 = 1) → (q' % 2 = 1) → (q' ∈ A'.step q σ )
+            → (q' ∈ A.to_1mod2.step q σ ) := by
+                intro q q' σ hq_odd hq'_odd hstep
+                subst hA'
+                simp [to_singular, hq_odd] at hstep ⊢
+                by_cases hacc : q ∈ (A.to_1mod2).accept ∧ σ = none
+                · simp [hacc] at hstep ⊢
+                  rcases hstep with h | h
+                  · exfalso
+                    simp[SingularAccept] at h
+                    omega
+                  · exact h
+                · simp [hacc] at hstep ⊢
+                  exact hstep
+
+               --transition between odds in A' -> same transition in A1
+
+            --next step: path between odds in A' is odd
+            --next step: odd path in A' -> odd path in A1
+
+            have path_to_singular_accept (q : ℕ) (y : List (Option α))
+                (h_q_1mod2: q % 2 = 1) (h_path : Nonempty (A'.Path q SingularAccept y)) :
+                ∃ qf mid, qf ∈ (A.to_1mod2).accept ∧ (Nonempty (A.to_1mod2.Path q qf mid)) ∧ y = mid ++ [none] := by
+                induction y generalizing q
+                case nil =>
+                    simp only [εNFA.isPath_nil] at h_path
+                    simp [SingularAccept] at h_path
+                    omega
+                case cons c tail h_induction =>
+                    obtain ⟨ h_path ⟩ := h_path
+                    cases h_path
+                    case cons t h_step h_path =>
+                        by_cases tail = []
+                        case pos h_tail_empty =>
+                            clear h_induction
+                            subst h_tail_empty
+                            replace h_path : Nonempty (A'.Path t SingularAccept []) := by use h_path
+                            simp only [εNFA.isPath_nil] at h_path
+                            subst h_path
+
+                            have h_c_none : c = none := by
+                                simp [hA', to_singular, h_q_1mod2] at h_step
+                                split_ifs at h_step
+                                case pos h_none => exact h_none.right
+                                case neg =>
+                                    have : SingularAccept % 2 = 1 :=
+                                        (A.to_1mod2.if_1mod2_step_is_1mod2 ⟨A,rfl⟩ q SingularAccept c h_step).right
+                                    simp [SingularAccept] at this -- contradiction
+                            subst h_c_none
+
+                            use q, []
+                            simp only [εNFA.isPath_nil, List.nil_append, and_self, and_true]
+
+                            simp [hA', to_singular, h_q_1mod2] at h_step
+                            split_ifs at h_step
+                            case pos h_q_accept => exact h_q_accept
+                            case neg =>
+                                have : SingularAccept % 2 = 1 :=
+                                        (A.to_1mod2.if_1mod2_step_is_1mod2 ⟨A,rfl⟩ q SingularAccept none h_step).right
+                                simp [SingularAccept] at this -- contradiction
+
+                        case neg h_tail_nonempty =>
+                            have h_t_1mod2 : t % 2 = 1 := by
+                                cases h_path
+                                case nil => contradiction
+                                case cons t' c' tail' h_step' h_path' =>
+                                    have h_t_not_SAS : t ≠ SingularAccept := by
+                                        by_contra!
+                                        subst this
+
+                                        have h_step'_empty : A'.step SingularAccept c' = ∅ := by
+                                            simp [hA', to_singular, SingularAccept, SingularStart]
+
+                                        simp [h_step'_empty] at h_step' --contradiction
+
+                                    simp [hA', to_singular, h_q_1mod2] at h_step
+                                    split_ifs at h_step
+                                    case pos h_accept =>
+                                        simp [h_t_not_SAS] at h_step
+                                        exact (A.to_1mod2.if_1mod2_step_is_1mod2 ⟨A, rfl⟩ q t c h_step).right
+                                    case neg => exact (A.to_1mod2.if_1mod2_step_is_1mod2 ⟨A, rfl⟩ q t c h_step).right
+
+                            replace h_path: Nonempty (A'.Path t SingularAccept tail) := by use h_path
+                            obtain ⟨ qf, mid', h_induction ⟩ := h_induction t h_t_1mod2 h_path
+                            use qf, c :: mid'
+                            simp [h_induction]
+                            replace h_induction := h_induction.right.left
+                            simp [hA', to_singular, h_q_1mod2] at h_step
+                            split_ifs at h_step
+                            case pos =>
+                                have : t ≠ SingularAccept := by simp [SingularAccept]; omega
+                                simp [this] at h_step
+                                apply A.to_1mod2.isPath_singleton.mpr at h_step
+                                exact A.to_1mod2.isPath_append.mpr ⟨ t, h_step, h_induction⟩
+                            case neg =>
+                                apply A.to_1mod2.isPath_singleton.mpr at h_step
+                                exact A.to_1mod2.isPath_append.mpr ⟨ t, h_step, h_induction⟩
+
+            replace h_path_s_accept: Nonempty (A'.Path s SingularAccept y') := by use h_path_s_accept
+            obtain ⟨qf, mid, h_qf_accept, h_mid_path, h_y'_eq⟩ :=
+              path_to_singular_accept (q := s) (y := y') first_transition_is_to_odd_state h_path_s_accept
+
+            have h_mid : mid.reduceOption = x := by
+                simp only [h_y'_eq, List.reduceOption_cons_of_none, List.reduceOption_append,
+                  List.reduceOption_nil, List.append_nil] at h_x'
+                exact h_x'
+
+            use s, qf, mid
+
+def εNFA.max_reachable_node (A : εNFA α ℕ) (n : ℕ) :=
+    (∃s₁: ℕ, ∃x: List (Option α), s₁ ∈ A.start ∧ Nonempty (A.Path s₁ n x))
+    ∧
+    ∀n': ℕ, (n' > n) → ¬(∃s₁: ℕ, ∃x: List (Option α), s₁ ∈ A.start ∧ Nonempty (A.Path s₁ n' x))
+
+def εNFA.is_finite_automata (A : εNFA α ℕ) :=
+    (A.start = ∅) ∨ (∃n: ℕ, A.max_reachable_node n)
+
+lemma if_1mod2_max_reachable_is_1mod2 (A : εNFA α ℕ) (n: ℕ) (hA: A.is_1mod2) (h_n: A.max_reachable_node n) :
+    n % 2 = 1 := by
+    unfold εNFA.max_reachable_node at h_n
+    obtain ⟨ ⟨ s, x, ⟨ h_s_start, h_path ⟩ ⟩, _ ⟩ := h_n
+    apply A.if_1mod2_qs_is_1mod2 hA at h_s_start
+    apply A.if_1mod2_path_is_same_mod2 hA s n x at h_path
+    omega
+
+lemma finite_iff_1mod2_is_finite (A : εNFA α ℕ) (A' : εNFA α ℕ) (hA': A' = A.to_1mod2) :
+    A.is_finite_automata ↔ A'.is_finite_automata := by
+    constructor
+    case mp =>
+        intro h_A_is_finite
+        unfold εNFA.is_finite_automata at h_A_is_finite ⊢
+        cases h_A_is_finite
+        case inl h_A_start_empty =>
+            left
+            simp [hA', εNFA.to_1mod2, h_A_start_empty]
+        case inr h_max_reachable =>
+            right
+            obtain ⟨ n, h_max_reachable ⟩ := h_max_reachable
+            use 2*n + 1
+            unfold εNFA.max_reachable_node at h_max_reachable ⊢
+            obtain ⟨ ⟨ s, x, ⟨ h_s_start, h_path ⟩ ⟩, h ⟩ := h_max_reachable
+            have h_A_path_iff_A'_path := (A.path_iff_1mod2_path A' s n (2*s + 1) (2*n + 1) x hA' rfl rfl).mp h_path
+            constructor
+            case left =>
+                use 2*s + 1, x
+                exact ⟨ by simp [hA', εNFA.to_1mod2, h_s_start], h_A_path_iff_A'_path ⟩
+            case right =>
+                intro k' h_k'
+                by_cases k' % 2 = 0
+                case pos h_k'_0mod2 =>
+                    simp
+                    intro s' h_s' x
+                    by_contra! h_A'_path
+
+                    replace h_s' := A'.if_1mod2_qs_is_1mod2 ⟨A, hA'⟩ s' h_s'
+                    have := A'.if_1mod2_path_is_same_mod2 ⟨A, hA'⟩ s' k' x h_A'_path
+                    omega
+
+                case neg =>
+                    let k := (k' - 1)/2
+
+                    have h_k_greater: k > n := by omega
+                    have h_path_A := h k h_k_greater
+                    simp at h_path_A ⊢
+                    intro s' h_s' x
+
+                    simp [hA', εNFA.to_1mod2] at h_s'
+                    obtain ⟨ s, h_s_start, h_s ⟩ := h_s'
+                    replace h_path_A := h_path_A s h_s_start x
+                    replace h_k': k' = 2*k + 1 := by omega
+                    by_contra! h_path_A'
+                    have := (A.path_iff_1mod2_path A' s k s' k' x hA' (symm h_s) h_k').mpr h_path_A'
+                    absurd h_path_A
+                    simp only [not_isEmpty_of_nonempty, not_false_eq_true]
+
+    case mpr =>
+        intro h_A'_is_finite
+        unfold εNFA.is_finite_automata at h_A'_is_finite ⊢
+        cases h_A'_is_finite
+        case inl h_A'_start_empty =>
+            left
+            by_contra! h_A_start_nonempty
+            obtain ⟨ q, h_q ⟩ := nonempty_def.mp h_A_start_nonempty
+            clear h_A_start_nonempty
+            absurd h_A'_start_empty
+            push_neg
+            simp [nonempty_def]
+            use 2*q + 1
+            simp [hA', εNFA.to_1mod2, h_q]
+
+        case inr h_max_reachable =>
+            right
+            obtain ⟨n', h_max_reachable⟩ := h_max_reachable
+            have h_n'_1mod2 : n' % 2 = 1 := if_1mod2_max_reachable_is_1mod2 A' n' ⟨A, hA'⟩ h_max_reachable
+
+            let n := (n' - 1) / 2
+            use n
+            unfold εNFA.max_reachable_node at h_max_reachable ⊢
+            constructor
+            case left =>
+                obtain ⟨ ⟨ s', x, ⟨ h_s'_start, h_A'_path ⟩ ⟩, _ ⟩ := h_max_reachable
+                simp [hA', εNFA.to_1mod2] at h_s'_start
+                obtain ⟨s, h_s ⟩ := h_s'_start
+                use s, x
+
+                refine ⟨ h_s.left, ?_ ⟩
+                have := A.path_iff_1mod2_path A' s n s' n' x hA' (symm h_s.right) (by omega)
+                exact this.mpr h_A'_path
+
+            case right =>
+                obtain ⟨ ⟨_ ⟩, h ⟩ := h_max_reachable
+                intro k h_k
+                let k' := k*2 + 1
+                simp
+                intro s h_s x
+                by_contra! h_path_A
+                have := h k' (by omega)
+                absurd this
+
+                let s' := s*2 + 1
+                have h_s'_start: s' ∈ A'.start := by
+                    simp [hA', εNFA.to_1mod2, s']
+                    use s
+                    exact ⟨h_s, by omega⟩
+
+                use s', x
+                refine ⟨ h_s'_start, ?_ ⟩
+                have := A.path_iff_1mod2_path A' s k s' k' x hA' (by omega) (by omega)
+                exact this.mp h_path_A
+
+lemma if_singular_1mod2_path (A A' : εNFA α ℕ) (qs qf : ℕ) (hA': A' = to_singular A)
+    (h_qs: qs % 2 = 1) (h_qf: qf % 2 = 1) (x: List (Option α)):
+    Nonempty (A'.Path qs qf x) ↔ Nonempty (A.to_1mod2.Path qs qf x) := by
+    constructor
+    case mp =>
+        intro h_A'_path
+        obtain ⟨ h_A'_path ⟩ := h_A'_path
+        induction h_A'_path
+        case nil => simp only [εNFA.isPath_nil]
+        case cons t qs qf c tail h_step h_path h_induction =>
+            have h_t : t % 2 = 1 := by
+                clear h_induction
+                by_contra!
+                simp [hA', to_singular, h_qs] at h_step
+                split_ifs at h_step
+                case pos h_c_none =>
+                    simp at h_step
+                    cases h_step
+                    case inl h_t_singular =>
+                        replace h_c_none := h_c_none.right
+                        subst h_c_none
+
+                        have h_t_step :∀ (c: Option α), A'.step t c = ∅ := by
+                            simp [h_t_singular, hA', to_singular, SingularAccept, SingularStart]
+
+                        cases h_path
+                        case nil => contradiction
+                        case cons t' c tail' h_step' _ =>
+                            replace h_t_step := h_t_step c
+                            simp [h_t_step] at h_step' -- contradiction
+
+                    case inr h_step =>
+                        have := A.to_1mod2.if_1mod2_step_is_1mod2 ⟨A, rfl⟩ qs t c h_step
+                        omega
+
+                case neg =>
+                    have := A.to_1mod2.if_1mod2_step_is_1mod2 ⟨A, rfl⟩ qs t c h_step
+                    omega
+
+            replace h_step : t ∈ A.to_1mod2.step qs c := by
+                simp [hA', to_singular, h_qs, SingularAccept, SingularStart] at h_step
+                split_ifs at h_step
+                case pos =>
+                    simp at h_step
+                    cases h_step
+                    case inl => omega
+                    case inr h_step=>  exact h_step
+                case neg => exact h_step
+
+            apply A.to_1mod2.isPath_singleton.mpr at h_step
+            have := h_induction h_t h_qf
+            exact A.to_1mod2.isPath_append.mpr ⟨ t, h_step, this ⟩
+
+    case mpr =>
+        intro h_A1mod2_path
+
+        have h_A'_contains_A_1mod2 : A'.contains A.to_1mod2 := by
+            subst hA'
+            exact to_singular_contains A
+
+        exact A'.path_if_contains A.to_1mod2 h_A'_contains_A_1mod2 qs qf x h_A1mod2_path
+
+lemma singular_path_from_odd_ends_odd
+    (A A' : εNFA α ℕ) (q qf : ℕ) (y : List (Option α))
+    (hA' : A' = to_singular A)
+    (h_q_odd : q % 2 = 1)
+    (h_qf_gt : qf > SingularStart)
+    (h_path : Nonempty (A'.Path q qf y)) :
+    qf % 2 = 1 := by
+  obtain ⟨ h_path ⟩ := h_path
+  induction h_path
+  · omega
+  · rename_i t q qf c tail h_step h_rest ih
+    by_cases h_tail_empty : tail = []
+    · subst h_tail_empty
+      replace h_rest : Nonempty (A'.Path t qf []) := by use h_rest
+      apply A'.isPath_nil.mp at h_rest
+
+      subst h_rest
+      have h_t_ne_zero : t ≠ SingularAccept := by
+        simp [SingularAccept]
+        omega
+
+      simp [hA', to_singular, h_q_odd, SingularAccept, SingularStart] at h_step h_t_ne_zero
+      split_ifs at h_step
+      · simp [h_t_ne_zero] at h_step
+        exact (A.to_1mod2.if_1mod2_step_is_1mod2 ⟨A, rfl⟩ q t c h_step).right
+      · exact (A.to_1mod2.if_1mod2_step_is_1mod2 ⟨A, rfl⟩ q t c h_step).right
+    · have h_t_odd : t % 2 = 1 := by
+        simp [hA', to_singular, h_q_odd] at h_step
+        split_ifs at h_step
+        · rcases h_step with h_zero | h_step1
+          · subst h_zero
+            cases h_rest with
+            | nil => contradiction
+            | cons =>
+                rename_i u d tail' hstep_bad hpath_bad
+                simp [hA', to_singular, SingularAccept, SingularStart] at hstep_bad
+          · exact (A.to_1mod2.if_1mod2_step_is_1mod2 ⟨A, rfl⟩ q t c h_step1).right
+        · exact (A.to_1mod2.if_1mod2_step_is_1mod2 ⟨A, rfl⟩ q t c h_step).right
+      exact ih h_t_odd h_qf_gt
+
+lemma finite_iff_to_singular_finite (A A' : εNFA α ℕ) (hA': A' = to_singular A):
+    A.is_finite_automata ↔ A'.is_finite_automata := by
+    rw [finite_iff_1mod2_is_finite A A.to_1mod2 rfl]
+
+    unfold εNFA.is_finite_automata
+    constructor
+    case mp =>
+        rintro (h_start_empty | h_max_reachable)
+        case inl =>
+            right
+
+            use SingularStart
+            unfold εNFA.max_reachable_node
+            constructor
+            case h.left =>
+                use SingularStart, []
+                simp [hA', to_singular]
+            case h.right =>
+                intro n' h_n'
+                by_contra!
+                obtain ⟨ s₁, x, h ⟩ := this
+                have : s₁ = SingularStart := by
+                    replace h := h.left
+                    simp [hA', to_singular] at h
+                    exact h
+                subst this
+                replace h := h.right
+                obtain ⟨ h ⟩ := h
+                cases h
+                case nil =>
+                    contradiction
+                case cons t c x' h_step h_path =>
+                    simp [hA', to_singular, h_start_empty, SingularStart] at h_step
+
+        case inr =>
+            right
+            obtain ⟨ n, h_n ⟩ := h_max_reachable
+
+            unfold εNFA.max_reachable_node at h_n ⊢
+
+            obtain ⟨ ⟨ q, x, h_q_start, h_path_q_n_x ⟩, h_n_max ⟩ := h_n
+
+            have h_A'_contains_A_1mod2 := to_singular_contains A
+            rw[← hA'] at h_A'_contains_A_1mod2
+
+            by_cases n > SingularStart
+            case pos =>
+                use n
+                constructor
+                case left =>
+                    use SingularStart, [none] ++ x
+                    refine ⟨ by simp [hA', to_singular], ?_ ⟩
+                    apply A'.path_if_contains A.to_1mod2 h_A'_contains_A_1mod2 at h_path_q_n_x
+
+                    have h_step: q ∈ A'.step SingularStart none := by
+                        simp [hA', to_singular, SingularStart, h_q_start]
+
+                    apply A'.isPath_singleton.mpr at h_step
+                    exact A'.isPath_append.mpr ⟨ q, h_step, h_path_q_n_x ⟩
+
+                case right =>
+                    intro n' h_n'
+
+                    simp at h_n_max ⊢
+                    intro s' h_s' x
+
+                    simp [hA', to_singular] at h_s'
+                    subst h_s'
+
+                    by_contra!
+                    obtain ⟨ this ⟩ := this
+                    cases this
+                    case nil =>
+                        omega
+                    case cons t' c tail h_step h_path =>
+                        have h_t_start: t' ∈ A.to_1mod2.start := by
+                            simp [hA', to_singular, SingularStart] at h_step
+                            exact h_step.right
+
+                        absurd h_n_max
+                        simp
+                        use n'
+                        have : n' > n := by omega
+                        simp [this]
+                        clear this
+
+                        use t'
+
+                        refine ⟨ h_t_start, ?_ ⟩
+                        use tail
+                        by_cases h_tail_empty: tail = []
+                        case pos =>
+                            subst h_tail_empty
+                            replace h_path : Nonempty (A'.Path t' n' []) := by use h_path
+                            simp [A'.isPath_nil] at h_path ⊢
+                            exact h_path
+                        case neg =>
+                            have h_t' : t' % 2 = 1 := A.to_1mod2.if_1mod2_qs_is_1mod2 ⟨A, rfl⟩ t' h_t_start
+                            have h_n' : n' % 2 = 1 := by
+                                clear h_step h_n_max h_t_start
+                                induction h_path
+                                case nil => omega
+                                case cons t t' n' c tail' h_step h_path h_induction =>
+                                    by_cases h_tail'_empty: tail' = []
+                                    case pos =>
+                                        subst h_tail'_empty
+                                        replace h_path : Nonempty (A'.Path t n' []) := by use h_path
+                                        simp at h_path
+                                        subst h_path
+                                        have : t ≠ SingularAccept := by
+                                            have : SingularStart > SingularAccept := by
+                                                simp [SingularStart, SingularAccept]
+                                            omega
+                                        simp [hA', to_singular, h_t'] at h_step
+                                        split_ifs at h_step
+                                        case pos =>
+                                            simp [this] at h_step
+                                            exact (A.to_1mod2.if_1mod2_step_is_1mod2 ⟨A, rfl⟩ t' t c h_step).right
+                                        case neg =>
+                                            exact (A.to_1mod2.if_1mod2_step_is_1mod2 ⟨A, rfl⟩ t' t c h_step).right
+
+                                    case neg =>
+                                        apply h_induction h_n' h_tail'_empty
+                                        simp [hA', to_singular, h_t'] at h_step
+                                        split_ifs at h_step
+                                        case pos h_accept =>
+                                            replace h_accept := h_accept.left
+                                            simp at h_step
+                                            cases h_step
+                                            case inl h_t_accept =>
+                                                subst h_t_accept
+                                                cases h_path
+                                                case nil => contradiction
+                                                case cons u c _ h_step _ =>
+                                                    simp [hA', to_singular, SingularAccept, SingularStart] at h_step -- contradiction
+
+                                            case inr h_step =>
+                                                exact (A.to_1mod2.if_1mod2_step_is_1mod2 ⟨A, rfl⟩ t' t c h_step).right
+                                        case neg =>
+                                            exact (A.to_1mod2.if_1mod2_step_is_1mod2 ⟨A, rfl⟩ t' t c h_step).right
+
+                            replace h_path : Nonempty (A'.Path t' n' tail) := by use h_path
+                            exact (if_singular_1mod2_path A A' t' n' hA' h_t' h_n' tail).mp h_path
+            case neg =>
+                use SingularStart
+                constructor
+                case left =>
+                    use SingularStart, []
+                    simp [hA', to_singular]
+                case right  h_n_less =>
+                    simp at h_n_less
+                    intro n' h_n'
+
+                    have h_not_reach : ¬ ∃ s₁ x, s₁ ∈ A.to_1mod2.start ∧ Nonempty (A.to_1mod2.Path s₁ n' x) := by
+                        exact h_n_max n' (by omega)
+
+                    rintro ⟨ q, x, h_q_start, h_A'_path ⟩
+                    have h_q : q = SingularStart := by
+                        simp [hA', to_singular] at h_q_start
+                        exact h_q_start
+                    subst h_q
+                    obtain ⟨ h_A'_path ⟩ := h_A'_path
+                    cases h_A'_path with
+                    | nil =>
+                        omega
+                    | cons =>
+                        rename_i t' σ tail hstep hpath
+                        replace hpath : Nonempty (A'.Path t' n' tail) := by use hpath
+                        have h_t_start : t' ∈ A.to_1mod2.start := by
+                            simp [hA', to_singular, SingularStart] at hstep
+                            exact hstep.2
+                        have h_t_odd : t' % 2 = 1 :=
+                            A.to_1mod2.if_1mod2_qs_is_1mod2 ⟨A, rfl⟩ t' h_t_start
+                        have h_n'_odd : n' % 2 = 1 := by
+                             exact singular_path_from_odd_ends_odd A A' t' n' tail hA' h_t_odd h_n' hpath
+                        have h_path_1mod2 : Nonempty (A.to_1mod2.Path t' n' tail) :=
+                            (if_singular_1mod2_path A A' t' n' hA' h_t_odd h_n'_odd tail).mp hpath
+
+                        exact h_not_reach ⟨ t', tail, h_t_start, h_path_1mod2 ⟩
+
+    case mpr =>
+        rintro (h_start_empty | h_max_reachable)
+        case inl =>
+            exfalso
+            rw [hA'] at h_start_empty
+            simp [to_singular] at h_start_empty
+        case inr =>
+            have h_A'_contains_A_1mod2 := to_singular_contains A
+            rw[← hA'] at h_A'_contains_A_1mod2
+
+            by_cases h_start_empty : A.to_1mod2.start = ∅
+            case pos =>
+                exact Or.inl h_start_empty
+            case neg =>
+                right
+                obtain ⟨n, h_n⟩ := h_max_reachable
+                unfold εNFA.max_reachable_node at h_n ⊢
+                obtain ⟨h_n_reachable, h_n_max⟩ := h_n
+                obtain ⟨s, x, h_s_start, h_path⟩ := h_n_reachable
+                have h_bound :
+                ∀ k s x, s ∈ A.to_1mod2.start → Nonempty (A.to_1mod2.Path s k x) → k ≤ n := by
+                    intro k s x h_s_start h_path_1mod2
+                    by_contra h_not_le
+                    have hk_gt : k > n := by omega
+                    have h_step_from_singular : s ∈ A'.step SingularStart none := by
+                        simp [hA', to_singular, SingularStart, h_s_start]
+                    have h_singleton : Nonempty (A'.Path SingularStart s [none]) := by
+                        apply A'.isPath_singleton.mpr
+                        exact h_step_from_singular
+                    have h_path_in_A' : Nonempty (A'.Path s k x) := by
+                        exact A'.path_if_contains A.to_1mod2 h_A'_contains_A_1mod2 s k x h_path_1mod2
+                    have h_reach_k_in_A' : Nonempty (A'.Path SingularStart k ([none] ++ x)) := by
+                        exact A'.isPath_append.mpr ⟨s, h_singleton, h_path_in_A'⟩
+                    have h_not_reach := h_n_max k hk_gt
+                    apply h_not_reach
+                    use SingularStart, [none] ++ x
+                    constructor
+                    · simp [hA', to_singular]
+                    · exact h_reach_k_in_A'
+                have h_nonempty : ∃ s, s ∈ A.to_1mod2.start := by
+                    by_contra h_no_s
+                    apply h_start_empty
+                    rw [Set.eq_empty_iff_forall_notMem]
+                    intro s hs
+                    exact h_no_s ⟨s, hs⟩
+                obtain ⟨s, h_s_start⟩ := h_nonempty
+
+                let R : ℕ → Prop :=
+                    fun k => ∃ s₁ x,
+                        s₁ ∈ A.to_1mod2.start ∧
+                        Nonempty (A.to_1mod2.Path s₁ k x)
+
+                have hR_nonempty_bounded : ∃ k ≤ n, R k := by
+                    use s
+                    constructor
+                    · exact h_bound s s [] h_s_start ((A.to_1mod2.isPath_nil).mpr rfl)
+                    · unfold R
+                      use s, []
+                      exact ⟨h_s_start, (A.to_1mod2.isPath_nil).mpr rfl⟩
+
+                let m := Nat.findGreatest R n
+
+                use m
+
+                constructor
+                · unfold m
+                  obtain ⟨k, hk_le_n, hk_R⟩ := hR_nonempty_bounded
+                  exact Nat.findGreatest_spec hk_le_n hk_R
+
+                · intro k hk
+                  by_contra h_reach_k
+
+                  have hk_le_n : k ≤ n := by
+                    obtain ⟨s₁, x, h_s₁_start, h_path⟩ := h_reach_k
+                    exact h_bound k s₁ x h_s₁_start h_path
+
+                  have h_not_reach_k : ¬ R k := by
+                    unfold m at hk
+                    exact Nat.findGreatest_is_greatest hk hk_le_n
+
+                  exact h_not_reach_k h_reach_k
